paxos/proof_helper.dfy
@@ -12,39 +12,39 @@ import opened Synod
 import opened Proof_Agreement_Invs
 
 
-lemma Lemma_DecidedImpliesQuorumOfAccepts(c:Constants, ds:DistrSys, idx:int) 
-    requires c.WF() && ds.WF(c)
-    requires c.ValidLdrIdx(idx) && LeaderHasDecided(c, ds, idx);
-    requires LdrAcceptsSetCorrespondToAcceptMsg(c, ds)
-    requires LeaderHasQuorumOfAccepts(c, ds, idx)
-    ensures exists qrm :: QuorumOfAcceptMsgs(c, ds, qrm, ds.leaders[idx].ballot)
-{
-    var l, b := ds.leaders[idx], ds.leaders[idx].ballot;
-    var qrm:set<Packet> := {};
-    var accepts := l.accepts;
-    var sentPackets := ds.network.sentPackets;
-    var i := 0;
-    while i < c.f + 1 
-        decreases c.f+1 - i
-        invariant |accepts| == c.f+1 - i
-        invariant |qrm| == i
-        invariant UniqueSources(qrm)
-        invariant forall s | s in accepts :: 
-            (forall p | p in qrm :: p.src != s)
-        invariant forall s | s in accepts :: s in l.accepts
-        invariant forall p | p in qrm :: p.msg.Accept?
-        invariant forall p | p in qrm :: p.msg.bal == b
-        invariant forall p | p in qrm :: p in sentPackets;
-        invariant forall p | p in qrm :: p.dst == Id(Ldr, idx);
-    {
-        var s :| s in accepts;
-        var pkt := Packet(s, Id(Ldr, idx), Accept(b));
-        qrm := qrm + {pkt};
-        accepts := accepts - {s};
-        i := i + 1;
-    }
-    assert QuorumOfAcceptMsgs(c, ds, qrm, b);
-}
+// lemma Lemma_DecidedImpliesQuorumOfAccepts(c:Constants, ds:DistrSys, idx:int) 
+//     requires c.WF() && ds.WF(c)
+//     requires c.ValidLdrIdx(idx) && LeaderHasDecided(c, ds, idx);
+//     requires LdrAcceptsSetCorrespondToAcceptMsg(c, ds)
+//     requires LeaderHasQuorumOfAccepts(c, ds, idx)
+//     ensures exists qrm :: QuorumOfAcceptMsgs(c, ds, qrm, ds.leaders[idx].ballot)
+// {
+//     var l, b, v := ds.leaders[idx], ds.leaders[idx].ballot, ds.leaders[idx].val;
+//     var qrm:set<Packet> := {};
+//     var accepts := l.accepts;
+//     var sentPackets := ds.network.sentPackets;
+//     var i := 0;
+//     while i < c.f + 1 
+//         decreases c.f+1 - i
+//         invariant |accepts| == c.f+1 - i
+//         invariant |qrm| == i
+//         invariant UniqueSources(qrm)
+//         invariant forall s | s in accepts :: 
+//             (forall p | p in qrm :: p.src != s)
+//         invariant forall s | s in accepts :: s in l.accepts
+//         invariant forall p | p in qrm :: p.msg.Accept?
+//         invariant forall p | p in qrm :: p.msg.bal == b
+//         invariant forall p | p in qrm :: p in sentPackets;
+//         invariant forall p | p in qrm :: p.dst == Id(Ldr, idx);
+//     {
+//         var s :| s in accepts;
+//         var pkt := Packet(s, Id(Ldr, idx), Accept(b, v));
+//         qrm := qrm + {pkt};
+//         accepts := accepts - {s};
+//         i := i + 1;
+//     }
+//     assert QuorumOfAcceptMsgs(c, ds, qrm, b);
+// }
 
 
 
